compiler/src/examples/TestFlatImp.v
@@ -53,19 +53,7 @@ Example fib(n: Z): stmt  :=
               (SOp _n Syntax.bopname.sub _n _one)))))
   )))).
 
-Instance myFlatImpParams: FlatImp.parameters := {|
-  FlatImp.syntax_params := myparams;
-  FlatImp.W := Words32Naive;
-  FlatImp.locals := Zkeyed_map word32;
-  FlatImp.env := Empty_set_keyed_map.map _;
-  FlatImp.mem := Mem;
-  FlatImp.locals_ok := @SortedList.map_ok (Zkeyed_map_params _) _;
-  FlatImp.env_ok := Empty_set_keyed_map.ok _;
-  FlatImp.mem_ok := @SortedList.map_ok DefaultMemImpl32.params _;
-  FlatImp.ext_spec t m action args outcome := False;
-  FlatImp.max_ext_call_code_size := Empty_set_rect _;
-  FlatImp.max_ext_call_code_size_nonneg := Empty_set_rect _;
-|}.
+Require Import compiler.Basic32Semantics.
 
 Definition eval_stmt_test fuel initialSt := eval_stmt map.empty fuel initialSt map.empty.
 
